proved correctness of validation on functions wrt subblock opsem, admitting well-formedness lemmas and symbolic execution can be weaken and strengthen.
git-svn-id: https://webdav.seas.upenn.edu/svn/sol/vol@2536 eef5ea85-cc2e-0410-bd84-0fae1f012da8

src/TV/symexe_correct.v
@@ -79,7 +79,38 @@ match (bs1, bs2) with
 | _ => False
 end.
 
-Variable lc0 : GVMap.
+Variable lc0 gl0 : GVMap.
+
+Definition tv_fdef (f1 f2:fdef) (gl:GVMap) :=
+match (f1, f2) with
+| (fdef_intro fh1 lb1, fdef_intro fh2 lb2) =>
+  fh1 = fh2 /\ tv_blocks lb1 lb2 lc0 gl
+end.
+
+Fixpoint tv_products (Ps1 Ps2:list product):=
+match (Ps1, Ps2) with
+| (nil, nil) => True
+| (product_fdec f1::Ps1', product_fdec f2::Ps2') => 
+  f1 = f2 /\ tv_products Ps1' Ps2'
+| (product_fdef f1::Ps1', product_fdef f2::Ps2') => 
+  tv_fdef f1 f2 gl0 /\ tv_products Ps1' Ps2'
+| (product_gvar gvar1::Ps1', product_gvar gvar2::Ps2') => 
+  gvar1 = gvar2 /\ tv_products Ps1' Ps2'
+| _ => False
+end.
+
+Definition tv_module (m1 m2:module) :=
+match (m1, m2) with
+| (module_intro TD1 Ps1, module_intro TD2 Ps2) =>
+  TD1 = TD2 /\ tv_products Ps1 Ps2
+end.
+
+Fixpoint tv_system (S1 S2:system) :=
+match (S1, S2) with
+| (nil, nil) => True
+| (m1::S1', m2::S2') => tv_module m1 m2 /\ tv_system S1' S2'
+| _ => False
+end.
 
 Inductive wf_subblock : subblock -> Prop :=
 | wf_subblock_intro : forall cs call0, 
@@ -93,106 +124,460 @@ Inductive wf_subblocks : list subblock -> Prop :=
   wf_subblocks sbs ->
   wf_subblocks (sb::sbs).
 
-Lemma tv_subblock__is__correct : forall S TD Ps 
-                            sb1 sb2 lc als gl lc' gl' tr Mem Mem' als',
+Inductive wf_block : block -> Prop :=
+| wf_block_intro : forall l ps sbs tmn, 
+  wf_subblocks sbs ->
+  wf_block (block_intro l ps sbs tmn).
+
+Lemma tv_terminator__is__correct : forall TD fh1 lb1 fh2 lb2 B1 B2 lc gl tmn B1' lc' tr,
+  tv_fdef (fdef_intro fh1 lb1) (fdef_intro fh2 lb2) gl0 ->
+  tv_block B1 B2 lc gl ->
+  dbTerminator TD (fdef_intro fh1 lb1) B1 lc gl tmn B1' lc' tr ->
+  exists B2', exists n,
+    tv_block B1' B2' lc gl /\
+    nth_error lb1 n = Some B1' /\
+    nth_error lb2 n = Some B2' /\
+    dbTerminator TD (fdef_intro fh2 lb2) B2 lc gl tmn B2' lc' tr.
+Proof.
+  intros TD fh1 lb1 fh2 lb2 B1 B2 lc gl tmn B1' lc' tr Htv_fdef Htv_block HdbTerminator.
+  inversion HdbTerminator; subst.
+    assert (exists B2', exists n, tv_block (block_intro l' ps' sbs' tmn') B2' lc gl /\ 
+                                  nth_error lb1 n = Some (block_intro l' ps' sbs' tmn') /\
+                                  nth_error lb2 n = Some B2') as J.
+      admit. (*lookup*)
+    destruct J as [B2' [n [J1 [J2 J3]]]].
+    exists B2'. exists n. split; auto. split; auto. split; auto.
+    destruct B2' as [l2' ps2' sbs2' tmn2'].
+    apply dbBranch with (c:=c); auto.
+      admit. (*lookup*)
+      admit. (*switch*)
+    
+    assert (exists B2', exists n, tv_block (block_intro l' ps' sbs' tmn') B2' lc gl /\ 
+                                  nth_error lb1 n = Some (block_intro l' ps' sbs' tmn') /\
+                                  nth_error lb2 n = Some B2') as J.
+      admit. (*lookup*)
+    destruct J as [B2' [n [J1 [J2 J3]]]].
+    exists B2'. exists n. split; auto. split; auto. split; auto.
+    destruct B2' as [l2' ps2' sbs2' tmn2'].
+    apply dbBranch_uncond; auto.
+      admit. (*lookup*)
+      admit. (*switch*)
+Qed.
+
+Definition tv_dbCall__is__correct_prop S1 TD Ps1 lc gl Mem0 call0 lc' gl' Mem' tr
+  (db:dbCall S1 TD Ps1 lc gl Mem0 call0 lc' gl' Mem' tr) :=
+  forall S2 Ps2,
+  tv_system S1 S2 ->
+  tv_products Ps1 Ps2 ->
+  dbCall S2 TD Ps2 lc gl Mem0 call0 lc' gl' Mem' tr.
+Definition tv_subblock__is__correct_prop S1 TD Ps1 lc als gl Mem sb1 lc' als' gl' Mem' tr
+  (db:dbSubblock S1 TD Ps1 lc als gl Mem sb1 lc' als' gl' Mem' tr) :=
+  forall S2 Ps2 sb2,
   uniq gl ->
   uniq lc ->
   wf_subblock sb2 ->
+  tv_system S1 S2 ->
+  tv_products Ps1 Ps2 ->
   tv_subblock sb1 sb2 lc gl ->
-  dbSubblock S TD Ps lc als gl Mem sb1 lc' als' gl' Mem' tr ->
-  dbSubblock S TD Ps lc als gl Mem sb2 lc' als' gl' Mem' tr.
-Proof.
-  intros S TD Ps sb1 sb2 lc als gl lc' gl' tr Mem0 Mem' als'
-         Huniqg Huniqc Wf Htv_subblock HdbSubblock.
-  inversion HdbSubblock; subst. clear HdbSubblock.
-  destruct sb2.
-  unfold tv_subblock in Htv_subblock.
-  simpl in Htv_subblock.
-  destruct Htv_subblock as [EQ1 EQ2]; subst.
-  inversion Wf; subst.
-  apply tv_cmds__is__correct with (cs':=l0) in H; eauto.
-Qed.
-
-Lemma tv_subblocks__is__correct : forall sbs1 S TD Ps 
-                            sbs2 lc als gl lc' gl' tr Mem Mem' als',
+  dbSubblock S2 TD Ps2 lc als gl Mem sb2 lc' als' gl' Mem' tr.
+Definition tv_subblocks__is__correct_prop S1 TD Ps1 lc als gl Mem sbs1 lc' als' gl' Mem' tr
+  (db:dbSubblocks S1 TD Ps1 lc als gl Mem sbs1 lc' als' gl' Mem' tr) :=
+  forall S2 Ps2 sbs2,
   uniq gl ->
   uniq lc ->
   wf_subblocks sbs2 ->
+  tv_system S1 S2 ->
+  tv_products Ps1 Ps2 ->
   tv_subblocks sbs1 sbs2 lc gl ->
-  dbSubblocks S TD Ps lc als gl Mem sbs1 lc' als' gl' Mem' tr ->
-  dbSubblocks S TD Ps lc als gl Mem sbs2 lc' als' gl' Mem' tr.
-Proof.
-  induction sbs1; intros S TD Ps sbs2 lc als gl lc' gl' tr Mem0 Mem' als' 
-                  Huniqg Huniqc Wf Htv_subblocks HdbSubblocks.
-  
-  destruct sbs2;try solve [auto | simpl in Htv_subblocks; inversion Htv_subblocks].
-  
-  destruct sbs2; simpl in Htv_subblocks; inversion Htv_subblocks.
-  clear Htv_subblocks.
-  inversion HdbSubblocks; subst. clear HdbSubblocks.
-  inversion Wf; subst. clear Wf.
-  apply tv_subblock__is__correct with (sb2:=s) in H10; auto.
-  apply IHsbs1 with (sbs2:=sbs2) in H16; eauto.
-    admit. (*uniq*)
-    admit. (*uniq*)
-    admit. (*tv inclusion*)
-Qed.
-
-Lemma tv_blocks__is__correct : forall S TD Ps gl lp lc n tmn1
-                            l1 ps1 sbs1 ps' l'
-                            lb1 lb2 lc' gl' tr Mem Mem' als' tmn' sbs1',
+  dbSubblocks S2 TD Ps2 lc als gl Mem sbs2 lc' als' gl' Mem' tr.
+Definition tv_block__is__correct_prop S1 TD Ps1 F1 arg state1 state2 tr
+  (db:dbBlock S1 TD Ps1 F1 arg state1 state2 tr) :=
+  forall S2 Ps2 fh1 lb1 fh2 lb2 B1 lc als gl Mem B1' lc' als' gl' Mem' B2,
+  state1 = mkState (mkEC B1 lc als) gl Mem ->
+  state2 = mkState (mkEC B1' lc' als') gl' Mem' ->
+  F1 = fdef_intro fh1 lb1 ->
+  uniq gl ->
+  uniq lc ->
+  wf_block B2 ->
+  tv_system S1 S2 ->
+  tv_products Ps1 Ps2 ->
+  tv_fdef (fdef_intro fh1 lb1) (fdef_intro fh2 lb2) gl0 ->
+  tv_block B1 B2 lc gl ->
+  exists B2', exists n,
+    dbBlock S2 TD Ps2 (fdef_intro fh2 lb2) arg 
+      (mkState (mkEC B2 lc als) gl Mem) 
+      (mkState (mkEC B2' lc' als') gl' Mem')
+      tr /\
+    nth_error lb1 n = Some B1' /\
+    nth_error lb2 n = Some B2' /\
+    tv_block B1' B2' lc gl.
+Definition tv_blocks__is__correct_prop S1 TD Ps1 F1 lp state1 state2 tr
+  (db:dbBlocks S1 TD Ps1 F1 lp state1 state2 tr) :=
+  forall S2 Ps2 fh1 lb1 fh2 lb2 gl lc n tmn1
+                            l1 ps1 sbs1 ps1' l1' als
+                            lc' gl' Mem Mem' als' tmn1' sbs1',
+  state1 = (mkState (mkEC (block_intro l1 ps1 sbs1 tmn1) lc als) gl Mem) ->
+  state2 = (mkState (mkEC (block_intro l1' ps1' sbs1' tmn1') lc' als') gl' Mem') ->
+  tv_system S1 S2 ->
+  tv_products Ps1 Ps2 ->
+  F1 = fdef_intro fh1 lb1 ->
+  tv_fdef (fdef_intro fh1 lb1) (fdef_intro fh2 lb2) gl0 ->
   tv_blocks lb1 lb2 lc gl ->
   nth_error lb1 n = Some (block_intro l1 ps1 sbs1 tmn1) ->
-  dbBlocks S TD Ps lp
-    (mkState (mkEC (block_intro l1 ps1 sbs1 tmn1) lc nil) gl Mem)
-    (mkState (mkEC (block_intro l' ps' sbs1' tmn') lc' als') gl' Mem')
-    tr ->
-  exists l2, exists ps2, exists sbs2, exists tmn2, exists sbs2',
+  exists l2, exists ps2, exists sbs2, exists tmn2, 
+  exists l2', exists ps2', exists sbs2', exists tmn2', exists n',
     nth_error lb2 n = Some (block_intro l2 ps2 sbs2 tmn2) /\
+    nth_error lb1 n' = Some (block_intro l1' ps1' sbs1' tmn1') /\
+    nth_error lb2 n' = Some (block_intro l2' ps2' sbs2' tmn2') /\
     tv_block (block_intro l1 ps1 sbs1 tmn1) (block_intro l2 ps2 sbs2 tmn2) lc gl /\
-    dbBlocks S TD Ps lp
-      (mkState (mkEC (block_intro l2 ps2 sbs2 tmn2) lc nil) gl Mem)
-      (mkState (mkEC (block_intro l' ps' sbs2' tmn') lc' als') gl' Mem')
-      tr /\ 
-    tv_subblocks sbs1' sbs2' lc gl.
-Admitted.
+    tv_block (block_intro l1' ps1' sbs1' tmn1') (block_intro l2' ps2' sbs2' tmn2') lc gl /\
+    dbBlocks S2 TD Ps2 (fdef_intro fh2 lb2) lp
+      (mkState (mkEC (block_intro l2 ps2 sbs2 tmn2) lc als) gl Mem)
+      (mkState (mkEC (block_intro l2' ps2' sbs2' tmn2') lc' als') gl' Mem')
+      tr.
+Definition tv_fdef__is__correct_prop fid rt lp S1 TD Ps1 lc gl Mem lc' gl' als' Mem' Rid oResult tr
+  (db:dbFdef fid rt lp S1 TD Ps1 lc gl Mem lc' gl' als' Mem' Rid oResult tr) :=
+  forall Ps2 S2 la lb1,
+  lookupFdefViaIDFromProducts Ps1 fid = Some (fdef_intro (fheader_intro rt fid la) lb1) ->
+  tv_system S1 S2 ->
+  tv_products Ps1 Ps2 ->
+  exists lb2,
+    lookupFdefViaIDFromProducts Ps2 fid = Some (fdef_intro (fheader_intro rt fid la) lb2) /\
+    tv_blocks lb1 lb2 lc gl /\
+    dbFdef fid rt lp S2 TD Ps2 lc gl Mem lc' gl' als' Mem' Rid oResult tr.
 
-Lemma tv_fdef__is__correct : forall TD Ps S1 S2 fid la lb1 lb2 lc gl lc' gl' als' Mem Mem' Rid oResult tr lp rt,
-  lookupFdefViaIDFromSystem S1 fid = Some (fdef_intro (fheader_intro rt fid la) lb1) ->
-  lookupFdefViaIDFromSystem S2 fid = Some (fdef_intro (fheader_intro rt fid la) lb2) ->
+Lemma tv_blocks_nth_Some_inv : forall lb1 lb2 lc gl n B1,
   tv_blocks lb1 lb2 lc gl ->
-  dbFdef fid rt lp S1 TD Ps lc gl Mem lc' gl' als' Mem' Rid oResult tr ->
-  dbFdef fid rt lp S2 TD Ps lc gl Mem lc' gl' als' Mem' Rid oResult tr.
+  nth_error lb1 n = Some B1 ->
+  exists B2, 
+    nth_error lb2 n = Some B2 /\ tv_block B1 B2 lc gl.
+Admitted. (*nth*)
+
+Lemma tv__is__correct :
+  (forall S1 TD Ps1 lc gl Mem0 call0 lc' gl' Mem' tr db, 
+     tv_dbCall__is__correct_prop S1 TD Ps1 lc gl Mem0 call0 lc' gl' Mem' tr db) /\
+  (forall S1 TD Ps1 lc als gl Mem sb1 lc' als' gl' Mem' tr db,
+     tv_subblock__is__correct_prop S1 TD Ps1 lc als gl Mem sb1 lc' als' gl' Mem' tr db) /\
+  (forall S1 TD Ps1 lc als gl Mem sbs1 lc' als' gl' Mem' tr db,
+     tv_subblocks__is__correct_prop S1 TD Ps1 lc als gl Mem sbs1 lc' als' gl' Mem' tr db) /\
+  (forall S1 TD Ps1 F1 arg state1 state2 tr db,
+     tv_block__is__correct_prop S1 TD Ps1 F1 arg state1 state2 tr db) /\
+  (forall S1 TD Ps1 F1 lp state1 state2 tr db,
+     tv_blocks__is__correct_prop S1 TD Ps1 F1 lp state1 state2 tr db) /\
+  (forall fid rt lp S1 TD Ps1 lc gl Mem lc' gl' als' Mem' Rid oResult tr db,
+     tv_fdef__is__correct_prop fid rt lp S1 TD Ps1 lc gl Mem lc' gl' als' Mem' Rid oResult tr db).
 Proof.
-  intros TD Ps S1 S2 fid la lb1 lb2 lc gl lc' gl' als' Mem0 Mem' Rid oResult tr lp rt
-         HlookupS1 HlookupS2 Htv_blocks HdbFdef.
-  inversion HdbFdef; subst; clear HdbFdef.
-    rewrite HlookupS1 in H. inversion H; subst. clear H.
-    
-    apply tv_blocks__is__correct with (n:=0)(lb1:=lb)(lb2:=lb2) in H1; auto.
-      destruct H1 as [l3 [ps3 [sbs3 [tmn3 [sbs2' [J1 [Htv_block [HdbBlocks Htv_subblocks]]]]]]]].
-      unfold tv_block in Htv_block. 
-      destruct Htv_block as [J2 [Htv_phinodes [Htv_subblocks' J3]]]; subst.
-      apply tv_subblocks__is__correct with (sbs2:=sbs2') in H2; auto.
-        assert (S1=S2) as Eq. admit.
-        subst.
-        apply dbFdef_func with (l1:=l3)(ps1:=ps3)(sbs1:=sbs3)(tmn1:=tmn3)(la:=la0)(lb:=lb2)
-          (lc1:=lc2)(gl1:=gl1)(Mem1:=Mem2)(als1:=als1)(l2:=l2)(ps2:=ps2)(sbs2:=sbs2'); auto.
-          clear - H0 J1 Htv_subblocks' Htv_phinodes Htv_blocks. admit.
+(db_mutind_cases
+  apply db_mutind with
+    (P  := tv_dbCall__is__correct_prop)
+    (P0 := tv_subblock__is__correct_prop)
+    (P1 := tv_subblocks__is__correct_prop)
+    (P2 := tv_block__is__correct_prop)
+    (P3 := tv_blocks__is__correct_prop)
+    (P4 := tv_fdef__is__correct_prop) Case);
+  unfold tv_dbCall__is__correct_prop, 
+         tv_subblock__is__correct_prop, tv_subblocks__is__correct_prop,
+         tv_block__is__correct_prop, tv_blocks__is__correct_prop,
+         tv_fdef__is__correct_prop; intros; subst.
+Case "dbCall_intro".
+  inversion d; subst.
+    apply H with (S2:=S2)(Ps2:=Ps2) in H2; auto.
+    clear H.
+    destruct H2 as [lb2 [J1 [J2 J3]]].
+    eauto.
 
-          admit. (*uniq*)
-          admit. (*uniq*)
-          admit. (*Wf*)
+    apply H with (S2:=S2)(Ps2:=Ps2) in H2; auto.
+    clear H.
+    destruct H2 as [lb2 [J1 [J2 J3]]].
+    eauto.
 
+Case "dbSubblock_intro".
+  destruct sb2.
+  unfold tv_subblock in H5.
+  simpl in H5.
+  destruct H5 as [EQ1 EQ2]; subst.
+  inversion H2; subst.
+  apply tv_cmds__is__correct with (cs':=l0) in d; eauto.
+
+Case "dbSubblocks_nil".
+  destruct sbs2;try solve [auto | simpl in H4; inversion H4].
+  
+Case "dbSubblocks_cons".
+  destruct sbs2; simpl in H6; inversion H6.
+  clear H6.
+  inversion H3; subst. clear H3.  
+  apply H with (S2:=S2)(Ps2:=Ps2) in H7; auto.
+  assert (tv_subblocks sbs sbs2 lc2 gl2) as J. 
+    admit. (*tv inclusion*)
+  apply H0 with (S2:=S2)(Ps2:=Ps2) in J; eauto.
+    admit. (*uniq*)
+    admit. (*uniq*)
+
+Case "dbBlock_intro".
+  inversion H0; subst. clear H0.
+  inversion H1; subst. clear H1.
+  destruct B2 as [l2 ps2 sbs2 tmn2].
+  unfold tv_block in H9.
+  destruct H9 as [EQ1 [Htv_phinodes [Htv_subblocks EQ2]]]; subst.
+  inversion H5; subst. clear H5.
+  assert (J:=Htv_subblocks).
+  apply H with (S2:=S2)(Ps2:=Ps2) in J; auto.
+  apply tv_terminator__is__correct with (B2:=block_intro l2 ps2 sbs2 tmn2)(fh2:=fh2)(lb2:=lb2) in d0; auto.
+    destruct d0 as [B2' [n [Htv_block1'2' [J2 [J3 Hdb]]]]].
+    exists B2'. exists n. 
+    split; eauto.
+    split; auto.
+    split; auto.
+      clear - Htv_block1'2'.
+      admit. (*tv inclusion*)
+
+    unfold tv_block.
+    split; auto.
+    split; auto.
+    split; auto.
+      clear - Htv_subblocks.
+      admit. (*tv inclusion*)      
+
+Case "dbBlocks_nil".
+  inversion H0; subst. clear H0.
+  apply tv_blocks_nth_Some_inv with (n:=n)(B1:=block_intro l1' ps1' sbs1' tmn1') in H5; auto.
+  destruct H5 as [[l2 ps2 sbs2 tmn2] [Hnth_error2 Htv_block]].
+  exists l2. exists ps2. exists sbs2. exists tmn2.
+  exists l2. exists ps2. exists sbs2. exists tmn2. 
+  exists n.
+  split; auto.
+
+Case "dbBlocks_cons".
+  inversion d; subst.
+  assert (J:=H7).  
+  apply tv_blocks_nth_Some_inv with (n:=n)(B1:=block_intro l1 ps1 sbs1 tmn1) in J; auto.
+  destruct J as [[l2 ps2 sbs2 tmn2] [Hnth_error2 Htv_block12]].
+  assert (J:=Htv_block12).
+  apply H with (S2:=S0)(Ps2:=Ps2)(fh3:=fh2)(lb3:=lb2)(fh2:=fh1)(lb2:=lb1)(Mem:=Mem0)(B1':=B')(lc':=lc3)(als':=als2)(gl':=gl2)(Mem':=Mem2)(als0:=als) in J; auto.
+    destruct J as [B2' [n' [Hdb [J1 [J2 Htv_block12']]]]].
+    clear H.
+    destruct B' as [l3 ps3 sbs3 tmn3].
+    assert (tv_blocks lb1 lb2 lc3 gl2) as H.
+      admit. (*tv inclusion*)      
+    apply H0 with (S2:=S0)(Ps2:=Ps2)(fh2:=fh1)(fh3:=fh2)(n:=n')(tmn1:=tmn3)
+      (l1:=l3)(ps1:=ps3)(sbs1:=sbs3)(ps1'0:=ps1')(l1'0:=l1')(als:=als2)(lc'0:=lc')(gl'0:=gl')
+      (Mem:=Mem2)(Mem'0:=Mem')(als'0:=als')(tmn1'0:=tmn1')(sbs1'0:=sbs1') in H; auto.
+    destruct H as [l4 [ps4 [sbs4 [tmn4 [l4' [ps4' [sbs4' [tmn4' [n'' [J3 [J4 [J5 [J6 [J7 J8]]]]]]]]]]]]]].
+    clear H0.
+    exists l2. exists ps2. exists sbs2. exists tmn2.
+    exists l4'. exists ps4'. exists sbs4'. exists tmn4'.
+    exists n''.
+    split; auto.
+    split; auto.
+    split; auto.
+    split; auto.
+    split.
+      clear - J7.
+      admit. (*tv inclusion*)      
+      
+      rewrite J2 in J3.
+      inversion J3; subst. clear J3.
+      eauto.
+
+    admit. (*uniq*)
+    admit. (*uniq*)
+    admit. (*Wf*)
+
+Case "dbFdef_func".
+    rewrite H1 in e. inversion e; subst. clear e.
+    assert (exists lb2, lookupFdefViaIDFromProducts Ps2 fid = Some (fdef_intro (fheader_intro rt fid la) lb2) /\
+                        tv_blocks lb lb2 lc gl) as J.
+      clear - H1 H3.
+      admit. (*lookup*)
+    destruct J as [lb2 [H4 H5]].
+    exists lb2. split; auto. split; auto.
+    assert (tv_blocks lb lb2 (initLocals la (params2GVs TD lp lc gl)) gl) as Htv_blocks.
+      clear - H5.
+      admit. (*tv inclusion*)      
+    apply H with (S2:=S2)(Ps2:=Ps2)(fh1:=fheader_intro rt fid la)(fh2:=fheader_intro rt fid la)(n:=0)
+      (ps1':=ps2)(l1':=l2)(als:=nil)(lc':=lc1)(gl':=gl1)
+      (Mem:=Mem0)(Mem':=Mem1)(als':=als1)(tmn1':=insn_return rid rt Result)(sbs1':=sbs2) 
+      (ps3:=ps1)(sbs3:=sbs1)(tmn2:=tmn1)(l3:=l1)in Htv_blocks; auto.
+      clear H.
+      destruct Htv_blocks as [l3 [ps3 [sbs3 [tmn2 [l2' [ps2' [sbs2' [tmn2' [n' [J1 [J2 [J3 [J4 [J5 J6]]]]]]]]]]]]]].
+
+      unfold tv_block in J5.
+      destruct J5 as [EQ [Htv_phinodes [Htv_subblocks EQ']]]; subst.
+      assert (tv_subblocks sbs2 sbs2' lc1 gl1) as Htv_subblocks'.
         clear - Htv_subblocks.
-        admit. (*tv inclusion*)
+        admit.
+      apply H0 with (S2:=S2)(Ps2:=Ps2) in Htv_subblocks'; auto.
+        clear H0.
+        apply dbFdef_func with (l1:=l3)(ps1:=ps3)(sbs1:=sbs3)(tmn1:=tmn2)(la:=la)(lb:=lb2)
+          (lc1:=lc1)(gl1:=gl1)(Mem1:=Mem1)(als1:=als1)(l2:=l2')(ps2:=ps2')(sbs2:=sbs2'); eauto.
+          rewrite <- J1. admit.
 
-        clear - Htv_blocks.
-        admit. (*tv inclusion*)
-        
-        clear - H0. admit.
+        admit. (*uniq*)
+        admit. (*uniq*)
+        admit. (*Wf*) 
 
-    admit. (*The other case*)
+      unfold tv_fdef.
+      split; auto.
+        clear - H5.
+        admit. (*tv inclusion*)      
+
+      rewrite <- e0.
+      admit.  (*nth*)
+
+Case "dbFdef_proc".
+    rewrite H1 in e. inversion e; subst. clear e.
+    assert (exists lb2, lookupFdefViaIDFromProducts Ps2 fid = Some (fdef_intro (fheader_intro rt fid la) lb2) /\
+                        tv_blocks lb lb2 lc gl) as J.
+      clear - H1 H3.
+      admit.  (*lookup*)
+    destruct J as [lb2 [H4 H5]].
+    exists lb2. split; auto. split; auto.
+    assert (tv_blocks lb lb2 (initLocals la (params2GVs TD lp lc gl)) gl) as Htv_blocks.
+      clear - H5.
+      admit. (*tv inclusion*)      
+    apply H with (S2:=S2)(Ps2:=Ps2)(fh1:=fheader_intro rt fid la)(fh2:=fheader_intro rt fid la)(n:=0)
+      (ps1':=ps2)(l1':=l2)(als:=nil)(lc':=lc1)(gl':=gl1)
+      (Mem:=Mem0)(Mem':=Mem1)(als':=als1)(tmn1':=insn_return_void rid)(sbs1':=sbs2) 
+      (ps3:=ps1)(sbs3:=sbs1)(tmn2:=tmn1)(l3:=l1)in Htv_blocks; auto.
+      clear H.
+      destruct Htv_blocks as [l3 [ps3 [sbs3 [tmn2 [l2' [ps2' [sbs2' [tmn2' [n' [J1 [J2 [J3 [J4 [J5 J6]]]]]]]]]]]]]].
+
+      unfold tv_block in J5.
+      destruct J5 as [EQ [Htv_phinodes [Htv_subblocks EQ']]]; subst.
+      assert (tv_subblocks sbs2 sbs2' lc1 gl1) as Htv_subblocks'.
+        clear - Htv_subblocks.
+        admit.
+      apply H0 with (S2:=S2)(Ps2:=Ps2) in Htv_subblocks'; auto.
+        clear H0.
+        apply dbFdef_proc with (l1:=l3)(ps1:=ps3)(sbs1:=sbs3)(tmn1:=tmn2)(la:=la)(lb:=lb2)
+          (lc1:=lc1)(gl1:=gl1)(Mem1:=Mem1)(als1:=als1)(l2:=l2')(ps2:=ps2')(sbs2:=sbs2'); auto.
+          rewrite <- J1. admit.
+
+        admit. (*uniq*)
+        admit. (*uniq*)
+        admit. (*Wf*) 
+
+      unfold tv_fdef.
+      split; auto.
+        clear - H5.
+        admit. (*tv inclusion*)      
+
+      rewrite <- e0.
+      admit. (*nth*)
+Qed.   
+
+Lemma tv_dbCall__is__correct : forall S1 TD Ps1 lc gl Mem0 call0 lc' gl' Mem' tr S2 Ps2,
+  dbCall S1 TD Ps1 lc gl Mem0 call0 lc' gl' Mem' tr ->
+  tv_system S1 S2 ->
+  tv_products Ps1 Ps2 ->
+  dbCall S2 TD Ps2 lc gl Mem0 call0 lc' gl' Mem' tr.
+Proof.
+  intros.
+  destruct tv__is__correct as [J _].
+  unfold tv_dbCall__is__correct_prop in J.
+  eapply J; eauto.
+Qed.
+
+Definition tv_subblock__is__correct : forall S1 TD Ps1 lc als gl Mem sb1 lc' als' gl' Mem' tr S2 Ps2 sb2,
+  dbSubblock S1 TD Ps1 lc als gl Mem sb1 lc' als' gl' Mem' tr ->
+  uniq gl ->
+  uniq lc ->
+  wf_subblock sb2 ->
+  tv_system S1 S2 ->
+  tv_products Ps1 Ps2 ->
+  tv_subblock sb1 sb2 lc gl ->
+  dbSubblock S2 TD Ps2 lc als gl Mem sb2 lc' als' gl' Mem' tr.
+Proof.
+  intros.
+  destruct tv__is__correct as [_ [J _]].
+  unfold tv_subblock__is__correct_prop in J.
+  eapply J; eauto.
+Qed.
+
+Lemma tv_subblocks__is__correct : forall S1 TD Ps1 lc als gl Mem sbs1 lc' als' gl' Mem' tr S2 Ps2 sbs2,
+  dbSubblocks S1 TD Ps1 lc als gl Mem sbs1 lc' als' gl' Mem' tr ->
+  uniq gl ->
+  uniq lc ->
+  wf_subblocks sbs2 ->
+  tv_system S1 S2 ->
+  tv_products Ps1 Ps2 ->
+  tv_subblocks sbs1 sbs2 lc gl ->
+  dbSubblocks S2 TD Ps2 lc als gl Mem sbs2 lc' als' gl' Mem' tr.
+Proof.
+  intros.
+  destruct tv__is__correct as [_ [_ [J _]]].
+  unfold tv_subblocks__is__correct_prop in J.
+  eapply J; eauto.
+Qed.
+
+Lemma tv_block__is__correct : forall S1 TD Ps1 arg tr
+  S2 Ps2 fh1 lb1 fh2 lb2 B1 lc als gl Mem B1' lc' als' gl' Mem' B2,
+  dbBlock S1 TD Ps1 (fdef_intro fh1 lb1) arg (mkState (mkEC B1 lc als) gl Mem) (mkState (mkEC B1' lc' als') gl' Mem') tr ->
+  uniq gl ->
+  uniq lc ->
+  wf_block B2 ->
+  tv_system S1 S2 ->
+  tv_products Ps1 Ps2 ->
+  tv_fdef (fdef_intro fh1 lb1) (fdef_intro fh2 lb2) gl0 ->
+  tv_block B1 B2 lc gl ->
+  exists B2', exists n,
+    dbBlock S2 TD Ps2 (fdef_intro fh2 lb2) arg 
+      (mkState (mkEC B2 lc als) gl Mem) 
+      (mkState (mkEC B2' lc' als') gl' Mem')
+      tr /\
+    nth_error lb1 n = Some B1' /\
+    nth_error lb2 n = Some B2' /\
+    tv_block B1' B2' lc gl.
+Proof.
+  intros.
+  destruct tv__is__correct as [_ [_ [_ [J _]]]].
+  unfold tv_block__is__correct_prop in J.
+  eapply J with (state1:=(mkState (mkEC B1 lc als) gl Mem0))(state2:=(mkState (mkEC B1' lc' als') gl' Mem'))(F1:=(fdef_intro fh1 lb1)); eauto.
+Qed.
+
+Lemma tv_blocks__is__correct : forall S1 TD Ps1 lp tr
+  S2 Ps2 fh1 lb1 fh2 lb2 gl lc n tmn1
+                            l1 ps1 sbs1 ps1' l1' als
+                            lc' gl' Mem Mem' als' tmn1' sbs1',
+  dbBlocks S1 TD Ps1 (fdef_intro fh1 lb1) lp (mkState (mkEC (block_intro l1 ps1 sbs1 tmn1) lc als) gl Mem) (mkState (mkEC (block_intro l1' ps1' sbs1' tmn1') lc' als') gl' Mem') tr ->
+  tv_system S1 S2 ->
+  tv_products Ps1 Ps2 ->
+  tv_fdef (fdef_intro fh1 lb1) (fdef_intro fh2 lb2) gl0 ->
+  tv_blocks lb1 lb2 lc gl ->
+  nth_error lb1 n = Some (block_intro l1 ps1 sbs1 tmn1) ->
+  exists l2, exists ps2, exists sbs2, exists tmn2, 
+  exists l2', exists ps2', exists sbs2', exists tmn2', exists n',
+    nth_error lb2 n = Some (block_intro l2 ps2 sbs2 tmn2) /\
+    nth_error lb1 n' = Some (block_intro l1' ps1' sbs1' tmn1') /\
+    nth_error lb2 n' = Some (block_intro l2' ps2' sbs2' tmn2') /\
+    tv_block (block_intro l1 ps1 sbs1 tmn1) (block_intro l2 ps2 sbs2 tmn2) lc gl /\
+    tv_block (block_intro l1' ps1' sbs1' tmn1') (block_intro l2' ps2' sbs2' tmn2') lc gl /\
+    dbBlocks S2 TD Ps2 (fdef_intro fh2 lb2) lp
+      (mkState (mkEC (block_intro l2 ps2 sbs2 tmn2) lc als) gl Mem)
+      (mkState (mkEC (block_intro l2' ps2' sbs2' tmn2') lc' als') gl' Mem')
+      tr.
+Proof.
+  intros.
+  destruct tv__is__correct as [_ [_ [_ [_ [J _]]]]].
+  unfold tv_blocks__is__correct_prop in J.
+  eapply J with (state1:=(mkState (mkEC (block_intro l1 ps1 sbs1 tmn1) lc als) gl Mem0))(state2:=(mkState (mkEC (block_intro l1' ps1' sbs1' tmn1') lc' als') gl' Mem'))(F1:=(fdef_intro fh1 lb1)); eauto.
+Qed.
+
+Lemma tv_fdef__is__correct : forall fid rt lp S1 TD Ps1 lc gl Mem lc' gl' als' Mem' Rid oResult tr
+  Ps2 S2 la lb1,
+  dbFdef fid rt lp S1 TD Ps1 lc gl Mem lc' gl' als' Mem' Rid oResult tr ->
+  lookupFdefViaIDFromProducts Ps1 fid = Some (fdef_intro (fheader_intro rt fid la) lb1) ->
+  tv_system S1 S2 ->
+  tv_products Ps1 Ps2 ->
+  exists lb2,
+    lookupFdefViaIDFromProducts Ps2 fid = Some (fdef_intro (fheader_intro rt fid la) lb2) /\
+    tv_blocks lb1 lb2 lc gl /\
+    dbFdef fid rt lp S2 TD Ps2 lc gl Mem lc' gl' als' Mem' Rid oResult tr.
+Proof.
+  intros.
+  destruct tv__is__correct as [_ [_ [_ [_ [_ J]]]]].
+  unfold tv_fdef__is__correct_prop in J.
+  eapply J; eauto.
 Qed.
 
 Extraction "symexe" tv_blocks.
